RUXt.lean
@@ -5,18 +5,21 @@ This is the root module; it imports the whole development.
 -/
 import RUXt.Lib.PMap
 import RUXt.Lib.List
+import RUXt.Lib.Telescopes
+import RUXt.Lang.Types
 import RUXt.Lang.Lang
+import RUXt.Lang.Library
 import RUXt.Lang.Semantics
-import RUXt.Lang.Assertion
-import RUXt.Model.TypeChecker
+import RUXt.Lang.TypeChecker
+import RUXt.Model.Assertion
 import RUXt.Model.Logic
-import RUXt.Model.RISL
+-- import RUXt.Model.RISL
 import RUXt.Model.Summary
 import RUXt.Model.Refute
-import RUXt.Types.Ty
-import RUXt.Types.Lib.Int
-import RUXt.Types.Lib.Bool
-import RUXt.Types.Lib.Unit
-import RUXt.Types.Lib.Own
-import RUXt.Types.Rules
-import RUXt.Types.Validity
+-- import RUXt.Types.Ty
+-- import RUXt.Types.Lib.Int
+-- import RUXt.Types.Lib.Bool
+-- import RUXt.Types.Lib.Unit
+-- import RUXt.Types.Lib.Own
+-- import RUXt.Types.Rules
+-- import RUXt.Types.Validity
