RUXt/Lang/Library.lean
@@ -1,0 +1,21 @@
+import RUXt.Lib.PMap
+import RUXt.Lang.Types
+import RUXt.Lang.Lang
+
+namespace RUXt
+
+/-- Function implementations. -/
+structure FunImpl where
+  params : List (PVar × Ty)
+  body : Expr
+  ty : Ty
+  paramsNodup : (params.map Prod.fst).Nodup
+
+/-- Libraries map function identifiers to their implementations. -/
+def Library := PMap Fid FunImpl
+
+/-- Get the implementation of a function by its identifier. -/
+def Library.get : Library → Fid → Option FunImpl
+  | Λ, f => Λ f
+
+end RUXt
