RUXt/Lang/Types.lean
@@ -1,0 +1,19 @@
+namespace RUXt
+
+/-- Base types for values. -/
+inductive BaseType
+  | int
+  | bool
+  | loc
+  | unit
+deriving DecidableEq
+
+/-- Identifiers for named types. -/
+abbrev Tid := String
+/-- Types: base types or named custom types. -/
+inductive Ty
+  | base (kind : BaseType)
+  | custom (name : Tid)
+deriving DecidableEq
+
+end RUXt
